@prefix : <http://gnafld.net/def/gnaf/> .
@prefix dc: <http://purl.org/dc/elements/1.1/> .
@prefix owl: <http://www.w3.org/2002/07/owl#> .
@prefix rdf: <http://www.w3.org/1999/02/22-rdf-syntax-ns#> .
@prefix xml: <http://www.w3.org/XML/1998/namespace> .
@prefix xsd: <http://www.w3.org/2001/XMLSchema#> .
@prefix rdfs: <http://www.w3.org/2000/01/rdf-schema#> .
@prefix skos: <http://www.w3.org/2004/02/skos/core#> .
@prefix dct: <http://purl.org/dc/terms/> .
@prefix vann: <http://purl.org/vocab/vann/> .
@prefix gnaf: <http://gnafld.net/def/gnaf/> .
@base <http://gnafld.net/def/gnaf> .

<http://gnafld.net/def/gnaf/GeocodeSubclassCollection> a skos:Collection ;
    skos:member
        :BuildingCentroidGeocode ,
        :CentreLineDroppedFrontageGeocode ,
        :DrivewayFrontageGeocode ,
        :EmergencyAccessGeocode ,
        :EmergencyAccessSecondaryGeocode ,
        :FrontDoorAccessGeocode ,
        :FrontageCentreGeocode ,
        :FrontageCentreSetbackGeocode ,
        :LetterboxGeocode ,
        :PropertyAccessPointGeocode ,
        :PropertyAccessPointSetbackGeocode ,
        :PropertyCentroidGeocode ,
        :PropertyCentroidManualGeocode ,
        :UnitCentroidGeocode ,
        :UnitCentroidManualGeocode ,
        :GapGeocode ,
        :WaterConnectionPointGeocode ,
        :WaterMeterGeocode ,
        :SewageConnectionPointGeocode ,
        :GasConnectionPointGeocode ,
        :GasMeterPointGeocode ,
        :TelephoneConnectionPointGeocode ,
        :ElectricityConnectionPointGeocode ,
        :ElectricityMeterPointGeocode ,
        :InternetConnectionPointGeocode ,
        :UnknownGeocode ,
        :StreetLocalityGeocode ,
        :LocalityGeocode
    ;
    skos:prefLabel "Geocode Subclasses Collection" .

# This ensures that an instance of a Geocode cannot be of more than one subclass
[
  rdf:type owl:AllDisjointClasses ;
  owl:members (
        :BuildingCentroidGeocode
        :CentreLineDroppedFrontageGeocode
        :DrivewayFrontageGeocode
        :EmergencyAccessGeocode
        :EmergencyAccessSecondaryGeocode
        :FrontDoorAccessGeocode
        :FrontageCentreGeocode
        :FrontageCentreSetbackGeocode
        :LetterboxGeocode
        :PropertyAccessPointGeocode
        :PropertyAccessPointSetbackGeocode
        :PropertyCentroidGeocode
        :PropertyCentroidManualGeocode
        :UnitCentroidGeocode
        :UnitCentroidManualGeocode
        :GapGeocode
        :WaterConnectionPointGeocode
        :WaterMeterGeocode
        :SewageConnectionPointGeocode
        :GasConnectionPointGeocode
        :GasMeterPointGeocode
        :TelephoneConnectionPointGeocode
        :ElectricityConnectionPointGeocode
        :ElectricityMeterPointGeocode
        :InternetConnectionPointGeocode
        :UnknownGeocode
        :StreetLocalityGeocode
        :LocalityGeocode
    ) ;
].

:BuildingAccessPointGeocode rdfs:subClassOf gnaf:Geocode , skos:Concept ;
    skos:prefLabel "Building Access Point"@en ;
    skos:definition "POINT OF ACCESS TO THE BUILDING"@en ;
    skos:altLabel "BAP"^^xsd:string ;
    dct:source "G-NAF Data Product Description, November 2017"^^xsd:string ;
    dct:countributor <http://orcid.org/0000-0002-8742-7730> ;
    rdfs:isDefinedBy <http://gnafld.net/def/gnaf/> .

:BuildingCentroidGeocode rdfs:subClassOf gnaf:Geocode , skos:Concept ;
    skos:prefLabel "Building Centroid"@en ;
    skos:definition "POINT AS CENTRE OF BUILDING AND LYING WITHIN ITS BOUNDS (E.G. FOR U-SHAPED BUILDING)"@en ;
    skos:altLabel "BC"^^xsd:string ;
    dct:source "G-NAF Data Product Description, November 2017"^^xsd:string ;
    dct:countributor <http://orcid.org/0000-0002-8742-7730> ;
    rdfs:isDefinedBy <http://gnafld.net/def/gnaf/> .

:CentreLineDroppedFrontageGeocode rdfs:subClassOf gnaf:Geocode , skos:Concept ;
    skos:prefLabel "Centre-Line Dropped Frontage"@en ;
    skos:definition "A POINT ON THE ROAD CENTRE-LINE OPPOSITE THE CENTRE OF THE ROAD FRONTAGE OF AN ADDRESS SITE"@en ;
    skos:altLabel CDF""^^xsd:string ;
    dct:source "G-NAF Data Product Description, November 2017"^^xsd:string ;
    dct:countributor <http://orcid.org/0000-0002-8742-7730> ;
    rdfs:isDefinedBy <http://gnafld.net/def/gnaf/> .

:DrivewayFrontageGeocode rdfs:subClassOf gnaf:Geocode , skos:Concept ;
    skos:prefLabel "Driveway Frontage"@en ;
    skos:definition "CENTRE OF DRIVEWAY ON ADDRESS SITE FRONTAGE"@en ;
    skos:altLabel "DF"^^xsd:string ;
    dct:source "G-NAF Data Product Description, November 2017"^^xsd:string ;
    dct:countributor <http://orcid.org/0000-0002-8742-7730> ;
    rdfs:isDefinedBy <http://gnafld.net/def/gnaf/> .

:EmergencyAccessGeocode rdfs:subClassOf gnaf:Geocode , skos:Concept ;
    skos:prefLabel "Emergency Access"@en ;
    skos:definition "SPECIFIC BUILDING OR PROPERTY ACCESS POINT FOR EMERGENCY SERVICES"@en ;
    skos:altLabel "EA"^^xsd:string ;
    dct:source "G-NAF Data Product Description, November 2017"^^xsd:string ;
    dct:countributor <http://orcid.org/0000-0002-8742-7730> ;
    rdfs:isDefinedBy <http://gnafld.net/def/gnaf/> .

:EmergencyAccessSecondaryGeocode rdfs:subClassOf gnaf:Geocode , skos:Concept ;
    skos:prefLabel "Emergency Access Secondary"@en ;
    skos:definition "SPECIFIC BUILDING OR PROPERTY SECONDARY ACCESS POINT FOR EMERGENCY SERVICES"@en ;
    skos:altLabel "EAS"^^xsd:string ;
    dct:source "G-NAF Data Product Description, November 2017"^^xsd:string ;
    dct:countributor <http://orcid.org/0000-0002-8742-7730> ;
    rdfs:isDefinedBy <http://gnafld.net/def/gnaf/> .

:FrontDoorAccessGeocode rdfs:subClassOf gnaf:Geocode , skos:Concept ;
    skos:prefLabel "Front Door Access"@en ;
    skos:definition "FRONT DOOR OF BUILDING"@en ;
    skos:altLabel "FDA"^^xsd:string ;
    dct:source "G-NAF Data Product Description, November 2017"^^xsd:string ;
    dct:countributor <http://orcid.org/0000-0002-8742-7730> ;
    rdfs:isDefinedBy <http://gnafld.net/def/gnaf/> .

:FrontageCentreGeocode rdfs:subClassOf gnaf:Geocode , skos:Concept ;
    skos:prefLabel "Frontage Centre"@en ;
    skos:definition "POINT ON THE CENTRE OF THE ADDRESS SITE FRONTAGE"@en ;
    skos:altLabel "FC"^^xsd:string ;
    dct:source "G-NAF Data Product Description, November 2017"^^xsd:string ;
    dct:countributor <http://orcid.org/0000-0002-8742-7730> ;
    rdfs:isDefinedBy <http://gnafld.net/def/gnaf/> .

:FrontageCentreSetbackGeocode rdfs:subClassOf gnaf:Geocode , skos:Concept ;
    skos:prefLabel "Frontage Centre Setback"@en ;
    skos:definition "A POINT SET BACK FROM THE CENTRE OF THE ROAD FRONTAGE WITHIN AN ADDRESS SITE"@en ;
    skos:altLabel "FCS"^^xsd:string ;
    dct:source "G-NAF Data Product Description, November 2017"^^xsd:string ;
    dct:countributor <http://orcid.org/0000-0002-8742-7730> ;
    rdfs:isDefinedBy <http://gnafld.net/def/gnaf/> .

:LetterboxGeocode rdfs:subClassOf gnaf:Geocode , skos:Concept ;
    skos:prefLabel "Letterbox"@en ;
    skos:definition "PLACE WHERE MAIL IS DEPOSITED"@en ;
    skos:altLabel "LB"^^xsd:string ;
    dct:source "G-NAF Data Product Description, November 2017"^^xsd:string ;
    dct:countributor <http://orcid.org/0000-0002-8742-7730> ;
    rdfs:isDefinedBy <http://gnafld.net/def/gnaf/> .

:PropertyAccessPointGeocode rdfs:subClassOf gnaf:Geocode , skos:Concept ;
    skos:prefLabel "Property Access Point"@en ;
    skos:definition "ACCESS POINT (CENTRE OF) AT THE ROAD FRONTAGE OF THE PROPERTY"@en ;
    skos:altLabel "PAP"^^xsd:string ;
    dct:source "G-NAF Data Product Description, November 2017"^^xsd:string ;
    dct:countributor <http://orcid.org/0000-0002-8742-7730> ;
    rdfs:isDefinedBy <http://gnafld.net/def/gnaf/> .

:PropertyAccessPointSetbackGeocode rdfs:subClassOf gnaf:Geocode , skos:Concept ;
    skos:prefLabel "Property Access Point Setback"@en ;
    skos:definition "A POINT SET BACK FROM THE (CENTRE OF THE) ACCESS POINT AT THE ROAD FRONTAGE OF THE PROPERTY"@en ;
    skos:altLabel "PAPS"^^xsd:string ;
    dct:source "G-NAF Data Product Description, November 2017"^^xsd:string ;
    dct:countributor <http://orcid.org/0000-0002-8742-7730> ;
    rdfs:isDefinedBy <http://gnafld.net/def/gnaf/> .

:PropertyCentroidGeocode rdfs:subClassOf gnaf:Geocode , skos:Concept ;
    skos:prefLabel "Property Centroid"@en ;
    skos:definition "POINT OF CENTRE OF PARCELS MAKING UP A PROPERTY AND LYING WITHIN ITS BOUNDARIES (E.G. FOR L-SHAPED PROPERTY)"@en ;
    skos:altLabel "PC"^^xsd:string ;
    dct:source "G-NAF Data Product Description, November 2017"^^xsd:string ;
    dct:countributor <http://orcid.org/0000-0002-8742-7730> ;
    rdfs:isDefinedBy <http://gnafld.net/def/gnaf/> .

:PropertyCentroidManualGeocode rdfs:subClassOf gnaf:Geocode , skos:Concept ;
    skos:prefLabel "Property Centroid Manual"@en ;
    skos:definition "POINT MANUALLY PLACED APPROXIMATELY AT CENTRE OF PARCELS MAKING UP A PROPERTY AND LYING WITHIN ITS BOUNDARIES (E.G. FOR L-SHAPED PROPERTY)"@en ;
    skos:altLabel "PCM"^^xsd:string ;
    dct:source "G-NAF Data Product Description, November 2017"^^xsd:string ;
    dct:countributor <http://orcid.org/0000-0002-8742-7730> ;
    rdfs:isDefinedBy <http://gnafld.net/def/gnaf/> .

:UnitCentroidGeocode rdfs:subClassOf gnaf:Geocode , skos:Concept ;
    skos:prefLabel "Unit Centroid"@en ;
    skos:definition "POINT AT CENTRE OF UNIT AND LYING WITHIN ITS BOUNDS (E.G. FOR U-SHAPED UNIT)"@en ;
    skos:altLabel "UC"^^xsd:string ;
    dct:source "G-NAF Data Product Description, November 2017"^^xsd:string ;
    dct:countributor <http://orcid.org/0000-0002-8742-7730> ;
    rdfs:isDefinedBy <http://gnafld.net/def/gnaf/> .

:UnitCentroidManualGeocode rdfs:subClassOf gnaf:Geocode , skos:Concept ;
    skos:prefLabel "Unit Centroid Manual"@en ;
    skos:definition "POINT MANUALLY PLACED APPROXIMATELY AT CENTRE OF UNIT AND LYING WITHIN ITS BOUNDS (E.G. FOR U-SHAPED UNIT)"@en ;
    skos:altLabel "UCM"^^xsd:string ;
    dct:source "G-NAF Data Product Description, November 2017"^^xsd:string ;
    dct:countributor <http://orcid.org/0000-0002-8742-7730> ;
    rdfs:isDefinedBy <http://gnafld.net/def/gnaf/> .

:GapGeocode rdfs:subClassOf gnaf:Geocode , skos:Concept ;
    skos:prefLabel "Gap Geocode"@en ;
    skos:definition "POINT PROGRAMMATICALLY ALLOCATED DURING THE G-NAF PRODUCTION PROCESS PROPORTIONALLY BETWEEN ADJACENT ADDRESS LOCATIONS (BASED ON NUMBER_FIRST)"@en ;
    skos:altLabel "GG"^^xsd:string ;
    dct:source "G-NAF Data Product Description, November 2017"^^xsd:string ;
    dct:countributor <http://orcid.org/0000-0002-8742-7730> ;
    rdfs:isDefinedBy <http://gnafld.net/def/gnaf/> .

:WaterConnectionPointGeocode rdfs:subClassOf gnaf:Geocode , skos:Concept ;
    skos:prefLabel "Water Connection Point"@en ;
    skos:definition "WATER CONNECTION POINT (E.G. BOX, OR UNDERGROUND CHAMBER)"@en ;
    skos:altLabel "WCP"^^xsd:string ;
    dct:source "G-NAF Data Product Description, November 2017"^^xsd:string ;
    dct:countributor <http://orcid.org/0000-0002-8742-7730> ;
    rdfs:isDefinedBy <http://gnafld.net/def/gnaf/> .

:WaterMeterGeocode rdfs:subClassOf gnaf:Geocode , skos:Concept ;
    skos:prefLabel "Water Meter"@en ;
    skos:definition "WATER METER POINT (E.G. BOX, OR UNDERGROUND CHAMBER)"@en ;
    skos:altLabel "WM"^^xsd:string ;
    dct:source "G-NAF Data Product Description, November 2017"^^xsd:string ;
    dct:countributor <http://orcid.org/0000-0002-8742-7730> ;
    rdfs:isDefinedBy <http://gnafld.net/def/gnaf/> .

:SewageConnectionPointGeocode rdfs:subClassOf gnaf:Geocode , skos:Concept ;
    skos:prefLabel "Sewage Connection Point"@en ;
    skos:definition "SEWERAGE CONNECTION POINT (E.G. BOX, OR UNDERGROUND CHAMBER)"@en ;
    skos:altLabel "SCP"^^xsd:string ;
    dct:source "G-NAF Data Product Description, November 2017"^^xsd:string ;
    dct:countributor <http://orcid.org/0000-0002-8742-7730> ;
    rdfs:isDefinedBy <http://gnafld.net/def/gnaf/> .

:GasConnectionPointGeocode rdfs:subClassOf gnaf:Geocode , skos:Concept ;
    skos:prefLabel "Gas Connection Point"@en ;
    skos:definition "GAS CONNECTION POINT (E.G. BOX, OR UNDERGROUND CHAMBER)"@en ;
    skos:altLabel "GCP"^^xsd:string ;
    dct:source "G-NAF Data Product Description, November 2017"^^xsd:string ;
    dct:countributor <http://orcid.org/0000-0002-8742-7730> ;
    rdfs:isDefinedBy <http://gnafld.net/def/gnaf/> .

:GasMeterPointGeocode rdfs:subClassOf gnaf:Geocode , skos:Concept ;
    skos:prefLabel "Gas Meter Point"@en ;
    skos:definition "GAS METER POINT (E.G. BOX, OR UNDERGROUND CHAMBER)"@en ;
    skos:altLabel "GM"^^xsd:string ;
    dct:source "G-NAF Data Product Description, November 2017"^^xsd:string ;
    dct:countributor <http://orcid.org/0000-0002-8742-7730> ;
    rdfs:isDefinedBy <http://gnafld.net/def/gnaf/> .

:TelephoneConnectionPointGeocode rdfs:subClassOf gnaf:Geocode , skos:Concept ;
    skos:prefLabel "Telephone Connection Point"@en ;
    skos:definition "TELEPHONE CONNECTION POINT (E.G. BOX, OR UNDERGROUND CHAMBER)"@en ;
    skos:altLabel "TCP"^^xsd:string ;
    dct:source "G-NAF Data Product Description, November 2017"^^xsd:string ;
    dct:countributor <http://orcid.org/0000-0002-8742-7730> ;
    rdfs:isDefinedBy <http://gnafld.net/def/gnaf/> .

:ElectricityConnectionPointGeocode rdfs:subClassOf gnaf:Geocode , skos:Concept ;
    skos:prefLabel "Electricity Connection Point"@en ;
    skos:definition "ELECTRICITY CONNECTION POINT (E.G. BOX, OR UNDERGROUND CHAMBER)"@en ;
    skos:altLabel "ECP"^^xsd:string ;
    dct:source "G-NAF Data Product Description, November 2017"^^xsd:string ;
    dct:countributor <http://orcid.org/0000-0002-8742-7730> ;
    rdfs:isDefinedBy <http://gnafld.net/def/gnaf/> .

:ElectricityMeterPointGeocode rdfs:subClassOf gnaf:Geocode , skos:Concept ;
    skos:prefLabel "Electricity Meter Point"@en ;
    skos:definition "ELECTRICITY METER POINT (E.G. BOX, OR UNDERGROUND CHAMBER)"@en ;
    skos:altLabel "EM"^^xsd:string ;
    dct:source "G-NAF Data Product Description, November 2017"^^xsd:string ;
    dct:countributor <http://orcid.org/0000-0002-8742-7730> ;
    rdfs:isDefinedBy <http://gnafld.net/def/gnaf/> .

:InternetConnectionPointGeocode rdfs:subClassOf gnaf:Geocode , skos:Concept ;
    skos:prefLabel "Internet Connection Point"@en ;
    skos:definition "INTERNET CONNECTION POINT (E.G. BOX, OR UNDERGROUND CHAMBER)"@en ;
    skos:altLabel "ICP^^xsd:string ;
    dct:source "G-NAF Data Product Description, November 2017"^^xsd:string ;
    dct:countributor <http://orcid.org/0000-0002-8742-7730> ;
    rdfs:isDefinedBy <http://gnafld.net/def/gnaf/> .

:UnknownGeocode rdfs:subClassOf gnaf:Geocode , skos:Concept ;
    skos:prefLabel "Unknown"@en ;
    skos:definition "THE TYPE OF REAL WORLD FEATURE THE POINT REPRESENTS IS NOT KNOWN"@en ;
    skos:altLabel "UNK"^^xsd:string ;
    dct:source "G-NAF Data Product Description, November 2017"^^xsd:string ;
    dct:countributor <http://orcid.org/0000-0002-8742-7730> ;
    rdfs:isDefinedBy <http://gnafld.net/def/gnaf/> .

:StreetLocalityGeocode rdfs:subClassOf gnaf:Geocode , skos:Concept ;
    skos:prefLabel "Street Locality"@en ;
    skos:definition "POINT REPRESENTING THE EXTENT OF A STREET WITHIN A LOCALITY"@en ;
    skos:altLabel "STL"^^xsd:string ;
    dct:source "G-NAF Data Product Description, November 2017"^^xsd:string ;
    dct:countributor <http://orcid.org/0000-0002-8742-7730> ;
    rdfs:isDefinedBy <http://gnafld.net/def/gnaf/> .

:LocalityGeocode rdfs:subClassOf gnaf:Geocode , skos:Concept ;
    skos:prefLabel "Locality"@en ;
    skos:definition "POINT REPRESENTING A LOCALITY"@en ;
    skos:altLabel "LOC"^^xsd:string ;
    dct:source "G-NAF Data Product Description, November 2017"^^xsd:string ;
    dct:countributor <http://orcid.org/0000-0002-8742-7730> ;
    rdfs:isDefinedBy <http://gnafld.net/def/gnaf/> .
