@prefix : <http://gnafld.net/def/gnaf/> .
@prefix dc: <http://purl.org/dc/elements/1.1/> .
@prefix owl: <http://www.w3.org/2002/07/owl#> .
@prefix rdf: <http://www.w3.org/1999/02/22-rdf-syntax-ns#> .
@prefix xml: <http://www.w3.org/XML/1998/namespace> .
@prefix xsd: <http://www.w3.org/2001/XMLSchema#> .
@prefix rdfs: <http://www.w3.org/2000/01/rdf-schema#> .
@prefix skos: <http://www.w3.org/2004/02/skos/core#> .
@prefix dct: <http://purl.org/dc/terms/> .
@prefix vann: <http://purl.org/vocab/vann/> .
@prefix gnaf: <http://gnafld.net/def/gnaf/> .
@base <http://gnafld.net/def/gnaf> .

<http://gnafld.net/def/gnaf/MeshBlockMatchSubclassCollection> a skos:Collection ;
    skos:member
        :ParcelLevelMatch ,
        :GapGeocodedAddressLevelMatch ,
        :StreetLocalityLevelSingleMatch ,
        :StreetLocalityLevelMultipleMatch ,
        :LocalityLevelSingleMatch
    ;
    skos:prefLabel "Mesh Block Match subclass Collection" .

# This ensures that an instance of a Mesh Block Match cannot be of more than one subclass
[
    a owl:AllDisjointClasses ;
    owl:members (
          :ParcelLevelMatch
          :GapGeocodedAddressLevelMatch
          :StreetLocalityLevelSingleMatch
          :StreetLocalityLevelMultipleMatch
          :LocalityLevelSingleMatch
      ) ;
].

:ParcelLevelMatch rdfs:subClassOf gnaf:MeshBlockMatch , skos:Concept ;
    skos:prefLabel "Parcel Level Match"@en ;
    skos:definition "A parcel level geocode for the address has been applied and clearly within the boundaries of a single mesh block. The mesh block ID allocated to the address in most cases is at a very high level of confidence."@en ;
    skos:altLabel "1"@en ;
    dct:source "G-NAF Data Product Description, November 2017"^^xsd:string ;
    dct:countributor <http://orcid.org/0000-0002-8742-7730> ;
    rdfs:isDefinedBy <http://gnafld.net/def/gnaf/> .

:GapGeocodedAddressLevelMatch rdfs:subClassOf gnaf:MeshBlockMatch , skos:Concept ;
    skos:prefLabel "Gap Geocoded Address Level Match"@en ;
    skos:definition "A gap geocoded match for the address has been applied and clearly within the boundaries of a single mesh block. The mesh block ID allocated to the address in most cases is at a high level of confidence."@en ;
    skos:altLabel "2"@en ;
    dct:source "G-NAF Data Product Description, November 2017"^^xsd:string ;
    dct:countributor <http://orcid.org/0000-0002-8742-7730> ;
    rdfs:isDefinedBy <http://gnafld.net/def/gnaf/> .

:StreetLocalityLevelSingleMatch rdfs:subClassOf gnaf:MeshBlockMatch , skos:Concept ;
    skos:prefLabel "Street Locality Level Single Match"@en ;
    skos:definition "A street-locality level geocode for the address has been applied and clearly within the boundaries of a single mesh block. The mesh block ID allocated to the address in most cases is at a high level of confidence."@en ;
    skos:altLabel "3"@en ;
    dct:source "G-NAF Data Product Description, November 2017"^^xsd:string ;
    dct:countributor <http://orcid.org/0000-0002-8742-7730> ;
    rdfs:isDefinedBy <http://gnafld.net/def/gnaf/> .

:StreetLocalityLevelMultipleMatch rdfs:subClassOf gnaf:MeshBlockMatch , skos:Concept ;
    skos:prefLabel "Street Locality Level Multiple Match"@en ;
    skos:definition "A street-locality level geocode for the address has been applied and is within the boundaries of a multiple mesh blocks. The mesh block ID allocated to the address is at a low level of confidence."@en ;
    skos:altLabel "4"@en ;
    dct:source "G-NAF Data Product Description, November 2017"^^xsd:string ;
    dct:countributor <http://orcid.org/0000-0002-8742-7730> ;
    rdfs:isDefinedBy <http://gnafld.net/def/gnaf/> .

:LocalityLevelSingleMatch rdfs:subClassOf gnaf:MeshBlockMatch , skos:Concept ;
    skos:prefLabel "Locality Level Single Match"@en ;
    skos:definition "A locality level geocode for the address has been applied and is within the boundaries of a multiple mesh blocks. The mesh block ID allocated to the address is at a very low level of confidence."@en ;
    skos:altLabel "5"@en ;
    dct:source "G-NAF Data Product Description, November 2017"^^xsd:string ;
    dct:countributor <http://orcid.org/0000-0002-8742-7730> ;
    rdfs:isDefinedBy <http://gnafld.net/def/gnaf/> .
